\documentclass[12pt]{article}

%useful packages
\usepackage{color,soul}
\usepackage[usenames,dvipsnames,svgnames,table]{xcolor}
\usepackage{amsmath,amsthm,amscd,amssymb,bm}
\usepackage{hyperref}
\hypersetup{
    colorlinks=true,
    linkcolor=JungleGreen
}
\usepackage[utf8]{inputenc}
\usepackage[top=2cm, bottom=3cm, left=2cm, right=2cm]{geometry}
\usepackage{pgfplots}
\usepackage{enumitem}
\usepgfplotslibrary{fillbetween}
\usetikzlibrary{patterns}
\usepackage{tcolorbox}
\usepackage{centernot}
\usepackage{mathtools}
\usepackage{xcolor}

%personal definitions and commands
\newcommand{\R}{\mathbb{R}} 
\newcommand{\E}{\mathbb{E}}
\newcommand{\V}{\mathbb{V}}
\newcommand{\C}{\mathbb{C}}
\newcommand{\Prob}{\mathbb{P}}
\newcommand{\e}{\epsilon}
\newcommand\numberthis{\addtocounter{equation}{1}\tag{\theequation}} %allows numbering of single equations in align* environment
\newcommand{\mtx}[1]{\ensuremath{\bm{\mathit{#1}}}}
\newcommand{\B}{\hat{\boldsymbol{\beta}}}
\newcommand{\Cov}{\mathbb{C}\text{ov}}
\newcommand{\N}{\mathcal{N}}



\title{ECON641 -- Problem Set 1}
\author{Anirudh Yadav}
\setlength\parindent{0pt}
\begin{document}

\maketitle

\setcounter{tocdepth}{1}
\tableofcontents

\newpage

\section{Warmup: factor intensity reversals}
First, I outline the small open economy environment of the $2\times 2$ HO model (for my own purposes). 
\begin{itemize}
\item Two goods, 1 and 2.
\item Two factors, $L$ and $K$; with endogenous factor prices $w$ and $r$, respectively.
\item Production technology is the same in both industries, but they may differ in their relative factor intensities.
\item Exogenously given goods prices, $p_1$ and $p_2$ (i.e. the demand side of the economy is pinned down).
\end{itemize}
Roughly speaking, `no factor intensity reversals' (NFIR) means the following: for any vector of factor prices $(w,r)$, the ordering of relative factor intensities in both industries is always the same. For example, in equilibrium the production of good 1 may be more capital intensive than production of good 2; NFIR implies that at any other vector of factor prices, the production of good 1 must always be more capital intensive compared to good 2. We can show that production technology exhibits NFIR if, given $p_1$ and $p_2$, equilibrium factor prices are uniquely pinned down.\\

\subsection{Cobb Douglas}

Cobb Douglas production clearly satisfies NFIR. To see this, suppose that $F_1(K_1,L_1) = AK_1^\alpha L_1^{1-\alpha}$ and $F_2(K_2,L_2) = AK_2^\beta L_2^{1-\beta}$. The first order conditions for the profit maximization problem for industry 1 are standard:
\begin{align}
p_1\alpha AK_1^{\alpha-1}L_1^{1-\alpha} &= r,\\
p_1(1-\alpha) AK_1^{\alpha}L_1^{-\alpha} &= w.
\end{align}
Dividing (2) by (1) gives
\begin{align}
\frac{1-\alpha}{\alpha} k_1 = \frac{w}{r} \implies k_1 = \frac{\alpha}{1-\alpha}\frac{w}{r}, \text{ where } k_1 = K_1/L_1
\end{align}
Now, the zero profit condition in industry 1 is
\begin{align}
rK_1 + w L_1 &= p_1  AK_1^\alpha L_1^{1-\alpha} \nonumber\\
\implies r k_1 + w &= p_1 A k_1^\alpha
\end{align}
Plugging (3) into (4) and rearranging gives
\begin{align}
p_1 = C_\alpha r^\alpha w^{1-\alpha}
\end{align}
where $C_\alpha = \frac{1}{A(1-\alpha)}\left(\frac{1-\alpha}{\alpha}\right)^\alpha$. An analogous derivation for industry 2 gives
\begin{align}
p_2 = C_\beta r^\beta w^{1-\beta}
\end{align}
where $C_\beta = \frac{1}{A(1-\beta)}\left(\frac{1-\beta}{\beta}\right)^\beta$.
Clearly, given $p_1$ and $p_2$, there is a unique solution to (5) and (6), $(w^*,r^*)$, (unless $\alpha = \beta$).\\

Another (perhaps more intuitive) way to establish NFIR would be to use equation (3) and the equivalent expression for industry 2. These expressions imply that in equilibrium:
\begin{align*}
\frac{k_1}{k_2} = \frac{\alpha (1-\beta)}{\beta(1-\alpha)}.
\end{align*}
That is, the relative factor intensities between the two industries is independent of factor prices.\\


\subsection{CES}

CES production \textit{does not} exhibit NFIR. To see this, suppose $F_i(K_i,L_i) = \left[K_i^{\frac{\sigma_i - 1}{\sigma_i}} + L_i^{\frac{\sigma_i - 1}{\sigma_i}}\right]^{\frac{\sigma_i}{\sigma_i - 1}}$ for $i = 1,2$. The FOCs for industry $i$ are
\begin{align}
p_i\left[K_i^{\frac{\sigma_i - 1}{\sigma_i}} + L_i^{\frac{\sigma_i - 1}{\sigma_i}}\right]^{\frac{1}{\sigma_i - 1}}K_i^{-1/\sigma_i} &= r \label{eq:ces1}\\
p_i\left[K_i^{\frac{\sigma_i - 1}{\sigma_i}} + L_i^{\frac{\sigma_i - 1}{\sigma_i}}\right]^{\frac{1}{\sigma_i - 1}}L_i^{-1/\sigma_i} &= w \label{eq:ces1}
\end{align}
Combining these expressions gives
\begin{align*}
k_i^{-1/\sigma_i} &= \frac{r}{w}\\
\implies k_i &= \left(\frac{r}{w}\right)^{-\sigma_i}.
\end{align*}
Thus, in equilibrium, the relative factor intensities between the two industries is
\begin{align*}
\frac{k_1}{k_2} = \left(\frac{r}{w}\right)^{\sigma_2-\sigma_1},
\end{align*}
which clearly depends on factor prices (unless $\sigma_1 = \sigma_2$).\\

\subsection{Leontief}

Clearly the Leontief production function exhibits NFIR. Suppose both industries have the same production function $F(K,L) = \min\{K,L\}$. Then in equilibrium, both industries must have $k_i = 1$. Then, relative factor intensities do not depend on factor prices. More generally, suppose $F_i(K_i,L_i) = \min\{\alpha_iK,\beta_iL\}$. Then in equilibrium, each industry's capital-labor ratio will be $k_i = \beta_i/\alpha_i$. Again, relative factor intensities are independent of factor prices.

\newpage

\section{$2 \times 2 \times 2$ HO Model}

\newpage

\section{Technology growth in a parameterized version of DFS}

\subsection{}
I follow the derivation in EK (2005). We are given the distribution of efficiencies for producing goods $j$ at Home and Foreign:
\begin{align*}
F_i(z)=\Pr[Z_i(j) \leq z ] = \exp(-T_iz^{-\theta})
\end{align*}

\iffalse
Now, if we pick some random $j \in [0,1]$, the probability distribution of its efficiency, $Z_i(j)$, is obviously same as above. Accordingly, we can order goods such that
\begin{align*}
j &= \exp(-T_iz_i(j)^{-\theta})\\
\implies z_i(j) &= \left(-\frac{T_i}{\ln j}\right)^{-1/\theta}.
\end{align*}
(Essentially, think of the index $j$ as the vertical axis of the CDF above).\\
\fi


Now, we want to derive the DFS-type $A(j)$ curve, which is defined as the ratio of $H$'s efficiency of producing $j$ to $F$'s corresponding efficiency.\\

In the EK setup the efficiencies are realizations of a random variable. Accordingly, we think of $j$ as the \textit{probability} that the $H$'s relative efficiency of producing $j$ is less than some number:
\begin{align*}
j &= \Pr\left[\frac{Z}{Z^*} \leq A\right]\\
&=\Pr\left[Z \leq AZ^*\right]\\
&= \int_0^\infty \exp(-T(Az_*)^{-\theta}) f(z_*)dz_*.
\end{align*}
Now,
\begin{align*}
f(z_*) = \frac{d}{dz} \exp(-T^*z^{-\theta}) = \theta T^*z^{-\theta-1}\exp(-T^*z^{-\theta})
\end{align*}
Substituting into the above integral gives
\begin{align*}
j &= T^*\int_0^\infty \exp(-T(Az_*)^{-\theta}) \times \theta z_*^{-\theta-1}\exp(-T^*z_*^{-\theta})dz_*\\
&=T^*\int_0^\infty \exp(-(TA^{-\theta}+T^*)z_*^{-\theta}) \times\theta z_*^{-\theta-1}dz_*\\
&= \frac{T^*}{(TA^{-\theta}+T^*)} \int_0^\infty \exp(-(TA^{-\theta}+T^*)z_*^{-\theta}) \times -\theta z_*^{-\theta-1}(TA^{-\theta}+T^*)dz_*\\
&=\frac{T^*}{(TA^{-\theta}+T^*)} \int_0^\infty \exp(-(TA^{-\theta}+T^*)z_*^{-\theta}) \times \theta z_*^{-\theta-1}(TA^{-\theta}+T^*)dz_*\\
&=\frac{T^*}{(TA^{-\theta}+T^*)},
\end{align*}
since $ \int_0^\infty \exp(-(TA^{-\theta}+T^*)z_*^{-\theta}) \times \theta z_*^{-\theta-1}(TA^{-\theta}+T^*)dz_* = 1$ (because it is the integral of the Frechet pdf with scale $(T^*A^{-\theta}+T)$). Thus, rearranging to get an expression for $A(j)$ gives
\begin{align}
A(j) = \left[\left(\frac{1-j}{j}\right)\frac{T^*}{T}\right]^{-1/\theta}. \label{eq:EK0}
\end{align}

\newpage

\subsection{}
First note that there are no trade costs so that $d_{ni} = 1$ for all $n,i \in \{F,H\}$.\\

Now, we know that within a country, goods will be purchased from the lowest cost source. Since Home has a comparative advantage at lower values of $j$, we know that Home will produce the range of goods $[0,\bar j]$ where
\begin{align*}
\frac{w}{z(\bar j)} = \frac{w^*}{z^*(\bar j)}.
\end{align*}
The LHS of the above expression is the unit cost of producing $\bar j$ at home, and the RHS is the cost of buying the good from Foreign. Rearranging the above expression gives
\begin{align}
\frac{z(\bar j)}{z^*(\bar j)} &= \frac{w}{w^*} \nonumber\\
\implies A(\bar j) &= \omega, \label{eq:EK1}
\end{align}
where $\omega = w/w^*$. Similarly, Foreign will produce a range of goods $[\underline j, 1]$ domestically, such that
\begin{align}
\frac{w^*}{z^*(\underline j)} &= \frac{w}{z(\underline j)} \nonumber \\
\implies A(\underline j) = \omega. \label{eq:EK2}
\end{align}
Thus, there is a unique cuttoff good.\\

Next, we need to invoke market clearing. Here, we note that preferences are Cobb Douglas, with equal weights across each good. Thus, each country spends a constant share of its income on each good. We know that Home produces $[0,\bar j]$ goods domestically, and exports $[0, \underline j]$ goods to Foreign. Thus, market clearing at Home requires
\begin{align}
wL = \bar j wL + \underline j w^*L^* \label{eq:EK3}\\
\end{align}
Substituting (\ref{eq:EK1}) and (\ref{eq:EK2}) into (\ref{eq:EK3}) and rearranging gives
\begin{align*}
L &= L A^{-1}(\omega) + \frac{1}{\omega} L^* A^{-1}(\omega)\\
\implies \frac{1}{A^{-1}(\omega)} &= 1 + \frac{1}{\omega} \frac{L^*}{L} 
\end{align*}
And, from the above derivation we know: $A^{-1}(\omega) = \frac{T^*}{(T\omega^{-\theta}+T^*)}$. Substituting this into the above expression gives
\begin{align*}
\frac{T\omega^{-\theta}+T^*}{T^*} &= 1 +\frac{1}{\omega} \frac{L^*}{L}\\
\implies \frac{T}{T^*} \omega^{-\theta} &=\frac{1}{\omega} \frac{L^*}{L}\\
\implies \omega &= \left[\frac{T^*}{T}\frac{L^*}{L}\right]^{1/(1-\theta)}.
\end{align*}
And the equilibrium cutoff good is
\begin{align*}
\bar j &= A^{-1}(\omega)
\end{align*}

\subsection{}
With no trade costs goods prices are identical in $H$ and $F$. Thus, $\omega$ measures $H$'s welfare relative to $F$'s. From the above expression for equilibrium $\omega$, if $\theta > 1$, then an increase in $T^*$ reduces relative welfare in $H$. The comparative static is
\begin{align*}
\frac{d\omega}{dT^*} = \left[\frac{1}{T}\frac{L^*}{L}\right]^{1/(1-\theta)} \frac{1}{1-\theta} (T^*)^{\theta/(1-\theta)}.
\end{align*}
So, if $\theta > 1$, then the effect of an increase in $T^*$ is decreasing in $L^*/L$, which is observable in the data.

\section{Key implications of EK's Ricardian model}

\subsection{}
The unit cost of sending good $j$ from $i$ to $n$ is given by
\begin{align}
C_{ni}(j) = \frac{c_i}{Z_i(j)}d_{ni} \label{eq:EK21}
\end{align}

\subsection{}
We want to compute the probability that $i$ will sell good $j$ to $n$. Since the derivation below is the same for all goods, I suppress the index $j$. \\

\textbf{(a)} From (\ref{eq:EK21}) note that 
\begin{align*}
Z_i = \frac{c_id_{ni}}{C_{ni}}
\end{align*}
Now,
\begin{align*}
\Pr[Z_i \leq p] &= \Pr[{c_id_{ni}}/{C_{ni}} \leq p]
\end{align*}
Thus,
\begin{align*}
\Pr[Z_i \leq {c_id_{ni}}/{p} ] &=  \Pr[{c_id_{ni}}/{C_{ni}} \leq {c_id_{ni}}/{p}]\\
&= \Pr[p \leq C_{ni}]\\
&= \Pr[C_{ni} \geq p]\\
&= 1- \Pr[C_{ni} \leq p]\\
\therefore \Pr[C_{ni} \leq p] &= 1-\Pr[Z_i \leq {c_id_{ni}}/{p} ]\\
&= 1- F_i(c_id_{ni}/{p})\\
&= 1- \exp(-T_i(c_id_{ni})^{-\theta}p^\theta),
\end{align*}
which is the probability distribution of $C_{ni}$. Denote this distribution as $G_{ni}$ so that
\begin{align}
G_{ni}(p) = 1- \exp(-T_i(c_id_{ni})^{-\theta}p^\theta) \label{eq:EK22}
\end{align}

\textbf{(b)} Next we want to compute the probability that $i$ is the cheapest supplier for $n$. Denote this probability as $\pi_{ni}$. We have
\begin{align}
\pi_{ni} \equiv \Pr[ C_{ni} &= \min\{C_{ns}; s\neq i\}] \nonumber \\
&= \Pr[C_{ns} \geq C_{ni} \text{ for all } s \neq i]\nonumber \\ 
&= \int_0^\infty \prod_{s\neq i}[1-G_{ns}(C_{ni})] dG_{ni}(C_{ni})\nonumber \\
&=  \int_0^\infty \prod_{s\neq i}[1-G_{ns}(p)] dG_{ni}(p), \label{eq:EK23}
\end{align}
where I just re-denote the integration dummy as $p$ to ease notation.\\

\textbf{(c)} Now,
\begin{align}
dG_{ni}(p) = \frac{d}{dp} G_{ni}(p) &= \exp(-T_i(c_id_{ni})^{-\theta}p^\theta) T_i(c_id_{ni})^{-\theta} \theta p^{\theta-1} \label{eq:EK24}
\end{align}
Substituting (\ref{eq:EK22}) and (\ref{eq:EK24}) into (\ref{eq:EK23}) gives
\begin{align*}
\pi_{ni} &= \int_0^\infty\left[ \prod_{s\neq i} \exp(-T_s(c_sd_{ns})^{-\theta}p^\theta) \right] \exp(-T_i(c_id_{ni})^{-\theta}p^\theta) T_i(c_id_{ni})^{-\theta} \theta p^{\theta-1}dp\\
&=  \int_0^\infty\exp(-\sum_{s \neq i} T_s(c_sd_{ns})^{-\theta}p^\theta)  \exp(-T_i(c_id_{ni})^{-\theta}p^\theta) T_i(c_id_{ni})^{-\theta} \theta p^{\theta-1}dp\\
&= \int_0^\infty\exp(-\sum_{i=1}^N T_i(c_{ni}d_{ni})^{-\theta}p^\theta)T_i(c_id_{ni})^{-\theta} \theta p^{\theta-1}dp\\
&=\int_0^\infty\exp(-\Phi_np^\theta) T_i(c_id_{ni}) \theta p^{\theta-1}dp\\
&=T_i(c_id_{ni})^{-\theta} \int_0^\infty\exp(-\Phi_np^\theta) \theta p^{\theta-1}dp\\
&= \frac{T_i(c_id_{ni})^{-\theta} }{\Phi_n} \int_0^\infty\exp(-\Phi_np^\theta) \Phi_n\theta p^{\theta-1}dp\\
&=\frac{T_i(c_id_{ni})^{-\theta} }{\Phi_n},
\end{align*}
since the integral in the second last line evaluates to 1, because it is a pdf of a probability distribution of the form (\ref{eq:EK22}).


\end{document}
